Add some basic proofs

policy_carrying_data/src/cell.rs
@@ -1,10 +1,15 @@
 use std::fmt::{Debug, Formatter};
 
 use policy_core::types::{Arithmetic, PrimitiveData};
+use policy_utils::random_u64;
 
 /// A cell that carries a value and a policy. For the evaluation semantics it is
-/// exactly the same as a `PrimitiveData` stored in `value`.
+/// exactly the same as a `PrimitiveData` stored in `value`. It more like a monad
+/// that carries a policy.
 pub struct Cell<T: PrimitiveData> {
+    /// A unique identifier for the policy.
+    id: u64,
+    /// The value that is stored in this cell.
     value: T,
     /// The policy that is used to determine how the value can be used and processed.
     policy: (),
@@ -30,6 +35,7 @@ where
         Self {
             value: T::zero(),
             policy: (),
+            id: random_u64(),
         }
     }
 
@@ -37,6 +43,7 @@ where
         Self {
             value: self.value.add(&_other.value),
             policy: (),
+            id: random_u64(),
         }
     }
 
@@ -44,6 +51,7 @@ where
         Self {
             value: self.value.div(&_other.value),
             policy: (),
+            id: random_u64(),
         }
     }
 
@@ -51,6 +59,7 @@ where
         Self {
             value: self.value.mul(&_other.value),
             policy: (),
+            id: random_u64(),
         }
     }
 
@@ -58,6 +67,7 @@ where
         Self {
             value: self.value.sub(&_other.value),
             policy: (),
+            id: random_u64(),
         }
     }
 }
