policy_proof/coq/types.v
@@ -1,54 +1,169 @@
-Require Import Coq.Numbers.BinNums.
 Require Import Coq.Strings.String.
+Require Import Coq.Lists.List.
+Require Import policy.
+
+(* A setoid is a set (X, ~) with an equivalence relation. *)
+(* We can derive three properties from an equivalence class:
+  1. Reflexivity.
+  2. Symmetry.
+  3. Transitivity.
+*)
+Require Import SetoidClass.
+Require Import RelationClasses.
 
 Inductive Conjuction: Type := And | Or.
+Inductive Comparison: Type := Gt | Lt | Ge | Le | Eq | Neq.
+Inductive BinaryOp: Type := Add | Sub | Mul | Div | Mod.
 
-(* Basic value types. *)
-Inductive Value: Set :=
-  | Integer: Z -> Value
-  | Bool: bool -> Value
-  | String: string -> Value
-  | NULL: Value.
+Inductive basic_type: Set :=
+  | IntegerType
+  | BoolType
+  | StringType.
+
+Definition type_matches (lhs rhs: basic_type): bool :=
+  match lhs, rhs with
+  | IntegerType, IntegerType => true
+  | BoolType, BoolType => true
+  | StringType, StringType => true
+  | _, _ => false
+  end.
+
+Definition type_to_coq_type (t: basic_type): Set :=
+  match t with
+  | IntegerType => nat
+  | BoolType => bool
+  | StringType => string
+  end.
 
 (* Attributes are themselves string representation of the name. *)
-Definition Attribute := string.
+Definition Attribute := (basic_type * string)%type.
 Definition Symbol := string.
 Definition Aggregate := string.
 
-(* Function types that can be applied on attributes *)
-Inductive Func: Type :=
-  (* Simply returns the value *)
-  | func_val: Value -> Func
-  (* Identity *)
-  | func_ident: Attribute -> Func
-  (* Function application *)
-  | func_expr: Symbol -> list Func -> Func.
-
-(* Aggregate types. *)
-Inductive Agg: Type :=
-  | agg_expr: Func -> Agg
-  | agg_agg: Aggregate -> Func -> Agg
-  | agg_func: Symbol -> list Agg -> Agg.
+Inductive transform_func : Set.
+Inductive aggregate_func : Set.
+Definition transform_list := list transform_func%type.
+Definition aggregate_list := list transform_func%type.
 
 (* Something that will appear in `where` or filter. *)
-Inductive Predicate (domain: Type): Type :=
+Inductive predicate (domain: Type): Type :=
   (* Constant true *)
-  | predicate_true: Predicate domain
+  | predicate_true: predicate domain
+  | predicate_false: predicate domain
   (* Negation *)
-  | predicate_not: Predicate domain -> Predicate domain
+  | predicate_not: predicate domain -> predicate domain
   (* A conjuction *)
-  | predicate_conj: Conjuction -> Predicate domain -> Predicate domain -> Predicate domain
+  | predicate_conj: Conjuction -> predicate domain -> predicate domain -> predicate domain
 .
 
-Definition true_to_coq_true (domain: Type) (p: Predicate domain): bool :=
+Definition true_to_coq_true (domain: Type) (p: predicate domain): bool :=
   match p with
   | predicate_true _ => true
   | _ => false
   end.
 
-Definition coq_true_to_true (domain: Type) (b: bool): Predicate domain :=
+Definition coq_true_to_true (domain: Type) (b: bool): predicate domain :=
   match b with
   | true => predicate_true domain
   | false => predicate_not domain (predicate_true domain)
   end.
 
+Module Cell.
+
+(* A cell that does not carry policies. *)
+Definition clean_cell: Set := basic_type % type.
+(* A cell that carries policies . *)
+Definition cell: Set := (clean_cell * policy) % type.
+
+End Cell.
+
+Module Schema.
+
+(* A distinction is made between the database schema, which specifies the structure
+of the database, and the database instance, which specifies its actual content:
+sets of tuples. *)
+
+(* A schema is a list of attributes. *)
+Definition schema: Set := (list Attribute)%type.
+
+End Schema.
+
+Module Tuple.
+
+(* A tuple is a list of cells of different values. *)
+Definition tuple_type: Set := (list Cell.cell)%type.
+
+(* A tuple is, in essence, an interpretation of abstract values to their
+concrete values. Thus it is a dependent type of `tuple_type`. We also
+make it a recursive type, so that we can build types of arbitrary length. *)
+Fixpoint tuple (ty: tuple_type): Set :=
+  match ty with
+  | nil => unit
+  | (bt, _) :: t' => (type_to_coq_type bt * policy) * tuple t'
+  end%type.
+
+Definition example_tuple_ty : tuple_type := (StringType, policy_empty) :: (BoolType, policy_empty) :: nil.
+Definition example_tuple: tuple example_tuple_ty := (("abcd"%string, policy_empty), ((true, policy_empty), tt)).
+Definition example_tuple_ty' : tuple_type := (IntegerType, policy_empty) :: nil.
+Definition example_tuple' : tuple example_tuple_ty' := ((1, policy_empty), tt).
+Definition example_tuple'' : tuple (example_tuple_ty' ++ example_tuple_ty) := 
+  ((1, policy_empty),
+    (("abcd"%string, policy_empty),
+      ((true, policy_empty),
+        tt))).
+
+(* A tuple type is a list of basic types. *)
+Fixpoint tuple_type_eq (ty1 ty2: tuple_type) : bool :=
+  match ty1, ty2 with
+    | nil, nil => true
+    | (bt1, _) :: t1', (bt2, _) :: t2' => andb (type_matches bt1 bt2) (tuple_type_eq t1' t2')
+    | _, _ => false
+  end.
+
+(* Useful for joining two databases tuple-wise. *)
+Definition tuple_concat (ty1 ty2: tuple_type)
+  (lhs: tuple ty1) (rhs: tuple ty2): tuple (ty1 ++ ty2).
+Proof.
+  intros.
+  induction ty1; auto.
+    (* Just use existing component to construct the given type. *)
+    simpl in *. destruct a; destruct lhs; constructor; auto.
+Defined.
+
+(* A tuple must equal *)
+Fixpoint tuple_eq (ty: tuple_type): forall (lhs rhs: tuple ty), Prop :=
+  match ty return (forall (lhs rhs: tuple ty), Prop) with
+    | nil => fun _ _ => True
+    | (h, p) :: tl => fun lhs rhs => 
+      (fst lhs) = (fst rhs) /\ (snd lhs) = (snd rhs) /\ tuple_eq tl (snd lhs) (snd rhs)
+  end. 
+
+Definition tuple_eq_eqv (ty: tuple_type): Equivalence (tuple_eq ty).
+Proof.
+  (* Note that `Equivalence` is a class. *)
+  split. 
+  - induction ty; simpl; auto.
+    destruct a. destruct c; simpl in *; auto.
+  - induction ty; simpl; auto. destruct a.
+    destruct c; simpl; split; destruct H; try rewrite H; intuition.
+  - unfold Transitive. intros. induction ty.
+    + auto.
+    + destruct a. destruct c;
+      simpl in *; intuition; try rewrite H1; try rewrite H; try rewrite H0; try rewrite H4; auto.
+Qed.
+
+Definition tuple_is_setoid (ty: tuple_type): Setoid (tuple ty).
+Proof.
+  exists (tuple_eq ty).
+  apply tuple_eq_eqv.
+Qed.
+
+Definition example_tuple_lhs : tuple example_tuple_ty := (("abcd"%string, policy_empty), ((true, policy_empty), tt)).
+Definition example_tuple_rhs : tuple example_tuple_ty := (("abcd"%string, policy_empty), ((true, policy_empty), tt)).
+
+Example example_tuple_eq: tuple_eq example_tuple_ty example_tuple_lhs example_tuple_lhs.
+Proof.
+  simpl. repeat split.
+Qed.
+
+End Tuple.
