policy_proof/coq/policy.v
@@ -1,0 +1,8 @@
+(* The policy library. *)
+
+(* For now, the policy is just a placeholder. *)
+Inductive policy : Set :=
+  | policy_empty : policy
+  | policy_select: policy
+  | policy_top : policy
+  .
